Proofs/mkEntries_correct.v
@@ -11,459 +11,459 @@ Module EntryProofsFn (Import G : Grammar.T).
   Module Import L := LemmasFn G.
   Module Export FollowProofs := FollowProofsFn G.
 
-Definition entries_correct es g :=
-  forall xp la,
-    In (xp, la) es
-    <-> In xp g.(prods)
-        /\ lookahead_for la (lhs xp) (rhs xp) g.
+  Definition entries_correct es g :=
+    forall xp la,
+      In (xp, la) es
+      <-> In xp g.(prods)
+          /\ lookahead_for la (lhs xp) (rhs xp) g.
 
-(* invariant relating a list of entries to a list of productions *)
-Definition entries_correct_wrt_productions es xps g :=
-  forall xp la,
-    In (xp, la) es <-> In xp xps /\ lookahead_for la (lhs xp) (rhs xp) g.
+  (* invariant relating a list of entries to a list of productions *)
+  Definition entries_correct_wrt_productions es xps g :=
+    forall xp la,
+      In (xp, la) es <-> In xp xps /\ lookahead_for la (lhs xp) (rhs xp) g.
 
-Lemma invariant_iff_entries_correct :
-  forall g es,
-    entries_correct_wrt_productions es g.(prods) g 
-    <-> entries_correct es g.
-Proof.
-  split; intros; auto.
-Qed.
+  Lemma invariant_iff_entries_correct :
+    forall g es,
+      entries_correct_wrt_productions es g.(prods) g 
+      <-> entries_correct es g.
+  Proof.
+    split; intros; auto.
+  Qed.
 
-Lemma empty_entries_correct_wrt_empty_productions :
-  forall g,
-    entries_correct_wrt_productions [] [] g.
-Proof.
-  intros g.
-  split; [intros Hin | intros [Hin _]]; inv Hin.
-Qed.
+  Lemma empty_entries_correct_wrt_empty_productions :
+    forall g,
+      entries_correct_wrt_productions [] [] g.
+  Proof.
+    intros g.
+    split; [intros Hin | intros [Hin _]]; inv Hin.
+  Qed.
 
-Lemma fromLookaheadList_preserves_prod :
-  forall xp xp' la las,
-    In (xp, la) (fromLookaheadList xp' las)
-    -> xp = xp'.
-Proof.
-  intros xp xp' la las Hin.
-  induction las as [| la' las]; simpl in *.
-  - inv Hin.
-  - inv Hin.
-    + inv H; auto.
-    + apply IHlas; auto.
-Qed.
+  Lemma fromLookaheadList_preserves_prod :
+    forall xp xp' la las,
+      In (xp, la) (fromLookaheadList xp' las)
+      -> xp = xp'.
+  Proof.
+    intros xp xp' la las Hin.
+    induction las as [| la' las]; simpl in *.
+    - inv Hin.
+    - inv Hin.
+      + inv H; auto.
+      + apply IHlas; auto.
+  Qed.
 
-Lemma entriesForProd_preserves_prod :
-  forall xp xp' la nu fi fo,
-    In (xp, la) (entriesForProd nu fi fo xp')
-    -> xp = xp'.
-Proof.
-  intros xp xp' la nu fi fo Hin.
-  unfold entriesForProd in Hin.
-  apply in_app_or in Hin.
-  destruct Hin; eapply fromLookaheadList_preserves_prod; eauto.
-Qed.
+  Lemma entriesForProd_preserves_prod :
+    forall xp xp' la nu fi fo,
+      In (xp, la) (entriesForProd nu fi fo xp')
+      -> xp = xp'.
+  Proof.
+    intros xp xp' la nu fi fo Hin.
+    unfold entriesForProd in Hin.
+    apply in_app_or in Hin.
+    destruct Hin; eapply fromLookaheadList_preserves_prod; eauto.
+  Qed.
 
-Lemma first_gamma_tail_first_gamma_cons :
-  forall g la x syms,
-    nullable_sym g (NT x)
-    -> first_gamma g la syms
-    -> first_gamma g la (NT x :: syms).
-Proof.
-  intros g la x syms Hnu Hfi.
-  induction Hfi.
-  apply FirstGamma with (gpre := NT x :: gpre); auto.
-Qed.
+  Lemma first_gamma_tail_first_gamma_cons :
+    forall g la x syms,
+      nullable_sym g (NT x)
+      -> first_gamma g la syms
+      -> first_gamma g la (NT x :: syms).
+  Proof.
+    intros g la x syms Hnu Hfi.
+    induction Hfi.
+    apply FirstGamma with (gpre := NT x :: gpre); auto.
+  Qed.
 
-Lemma first_gamma_terminal_head :
-  forall g la y syms,
-    first_gamma g la (T y :: syms)
-    -> la = LA y.
-Proof.
-  intros g la y syms Hfi.
-  pose proof Hfi as Hfi'.
-  inv Hfi.
-  destruct gpre; simpl in *.
-  - inv H.
-    inv H2; auto.
-  - inv H.
-    exfalso.
-    eapply gamma_with_terminal_not_nullable with
-        (gpre := nil)
-        (y := y)
-        (gsuf := gpre); eauto.
-Qed.
+  Lemma first_gamma_terminal_head :
+    forall g la y syms,
+      first_gamma g la (T y :: syms)
+      -> la = LA y.
+  Proof.
+    intros g la y syms Hfi.
+    pose proof Hfi as Hfi'.
+    inv Hfi.
+    destruct gpre; simpl in *.
+    - inv H.
+      inv H2; auto.
+    - inv H.
+      exfalso.
+      eapply gamma_with_terminal_not_nullable with
+          (gpre := nil)
+          (y := y)
+          (gsuf := gpre); eauto.
+  Qed.
 
-Lemma first_gamma_head_or_tail :
-  forall g la sym syms,
-    first_gamma g la (sym :: syms)
-    -> first_sym g la sym
-       \/ (nullable_sym g sym
-           /\ first_gamma g la syms).
-Proof.
-  intros g la sym syms Hfi.
-  pose proof Hfi as Hfi'.
-  inv Hfi.
-  destruct gpre; simpl in *.
-  - inv H; auto.
-  - inv H.
-    right.
-    split.
-    + inv H0; auto.
-    + inv H0.
-      apply FirstGamma with (gpre := gpre); auto.
-Qed.
+  Lemma first_gamma_head_or_tail :
+    forall g la sym syms,
+      first_gamma g la (sym :: syms)
+      -> first_sym g la sym
+         \/ (nullable_sym g sym
+             /\ first_gamma g la syms).
+  Proof.
+    intros g la sym syms Hfi.
+    pose proof Hfi as Hfi'.
+    inv Hfi.
+    destruct gpre; simpl in *.
+    - inv H; auto.
+    - inv H.
+      right.
+      split.
+      + inv H0; auto.
+      + inv H0.
+        apply FirstGamma with (gpre := gpre); auto.
+  Qed.
 
-Lemma firstGamma_sound :
-  forall g la nu fi gamma,
-    nullable_set_for nu g
-    -> first_map_for fi g
-    -> In la (firstGamma' gamma nu fi)
-    -> first_gamma g la gamma.
-Proof.
-  intros g la nu fi gamma Hns Hfm Hin.
-  induction gamma as [| sym syms]; simpl in *.
-  - inv Hin.
-  - destruct sym as [y | x].
-    + inv Hin.
-      * apply FirstGamma with (gpre := nil); auto.
-      * inv H.
-    + destruct (NtSet.mem x nu) eqn:Hmem.
-      * destruct (NtMap.find x fi) as [fiSet |] eqn:Hfind.
-        -- apply in_app_or in Hin.
-           inv Hin.
-           ++ destruct Hfm as [Hsou Hcom].
-              unfold first_map_sound in Hsou.
-              apply Hsou with (la := la) in Hfind.
-              ** apply FirstGamma with (gpre := nil); auto.
-              ** apply in_elements_iff_in_laSet; auto.
-           ++ apply first_gamma_tail_first_gamma_cons; auto.
-              destruct Hns as [Hsou Hcom].
-              apply Hsou.
-              apply NtSet.mem_spec; auto.
-        -- simpl in *.
-           apply first_gamma_tail_first_gamma_cons; auto.
-           destruct Hns as [Hsou Hcom].
-           apply Hsou.
-           apply NtSet.mem_spec; auto.
-      * destruct (NtMap.find x fi) as [fiSet |] eqn:Hfind.
-        -- destruct Hfm as [Hsou com].
-           eapply Hsou in Hfind.
-           apply FirstGamma with (gpre := nil); auto.
-           apply Hfind.
-           apply in_elements_iff_in_laSet; auto.
-        -- inv Hin.
-Qed.
-
-(* There's probably a way to shorten this *)
-Lemma firstGamma_complete :
+  Lemma firstGamma_sound :
     forall g la nu fi gamma,
-    nullable_set_for nu g
-    -> first_map_for fi g
-    -> first_gamma g la gamma
-    -> In la (firstGamma' gamma nu fi).
-Proof.
-  intros g la nu fi gamma Hnu Hfm Hfg.
-  induction gamma as [| sym syms].
-  - simpl in *.
-    inv Hfg. (* LEMMA *)
-    symmetry in H.
-    apply app_cons_not_nil in H; inv H.
-  - destruct sym as [y | x]; simpl in *.
-    + apply first_gamma_terminal_head in Hfg; auto.
-    + destruct (NtSet.mem x nu) eqn:Hmem.
-      * (* x is in the nullable set, so we know it's nullable *)
-        destruct (NtMap.find x fi) as [fiSet |] eqn:Hfind.
-        -- apply in_or_app.
-           apply first_gamma_head_or_tail in Hfg.
-           inv Hfg.
-           ++ destruct Hfm as [Hsou Hcom].
-              eapply Hcom in H.
-              destruct H as [fiSet' [Hnf Hlin]]; auto.
-              left.
-              assert (fiSet = fiSet') by congruence; subst.
+      nullable_set_for nu g
+      -> first_map_for fi g
+      -> In la (firstGamma' gamma nu fi)
+      -> first_gamma g la gamma.
+  Proof.
+    intros g la nu fi gamma Hns Hfm Hin.
+    induction gamma as [| sym syms]; simpl in *.
+    - inv Hin.
+    - destruct sym as [y | x].
+      + inv Hin.
+        * apply FirstGamma with (gpre := nil); auto.
+        * inv H.
+      + destruct (NtSet.mem x nu) eqn:Hmem.
+        * destruct (NtMap.find x fi) as [fiSet |] eqn:Hfind.
+          -- apply in_app_or in Hin.
+             inv Hin.
+             ++ destruct Hfm as [Hsou Hcom].
+                unfold first_map_sound in Hsou.
+                apply Hsou with (la := la) in Hfind.
+                ** apply FirstGamma with (gpre := nil); auto.
+                ** apply in_elements_iff_in_laSet; auto.
+             ++ apply first_gamma_tail_first_gamma_cons; auto.
+                destruct Hns as [Hsou Hcom].
+                apply Hsou.
+                apply NtSet.mem_spec; auto.
+          -- simpl in *.
+             apply first_gamma_tail_first_gamma_cons; auto.
+             destruct Hns as [Hsou Hcom].
+             apply Hsou.
+             apply NtSet.mem_spec; auto.
+        * destruct (NtMap.find x fi) as [fiSet |] eqn:Hfind.
+          -- destruct Hfm as [Hsou com].
+             eapply Hsou in Hfind.
+             apply FirstGamma with (gpre := nil); auto.
+             apply Hfind.
              apply in_elements_iff_in_laSet; auto.
-           ++ destruct H.
-              right; auto.
-        -- simpl.
-           apply IHsyms.
-           apply first_gamma_head_or_tail in Hfg.
-           inv Hfg.
-           ++ destruct Hfm as [Hsou Hcom].
-              eapply Hcom in H.
-              destruct H as [fiSet' [Hnf Hli]]; auto.
-              congruence.
-           ++ destruct H; auto.
-      * destruct (NtMap.find x fi) as [fiSet |] eqn:Hfind.
-        -- apply first_gamma_head_or_tail in Hfg.
-           inv Hfg.
-           ++ destruct Hfm as [Hsou Hcom].
-              eapply Hcom in H.
-              destruct H as [fiSet' [Hnf Hli]]; auto.
-              assert (fiSet = fiSet') by congruence; subst.
-              apply in_elements_iff_in_laSet; auto.
-           ++ destruct H.
-              destruct Hnu as [Hsou Hcom].
-              apply Hcom in H.
-              rewrite <- NtSet.mem_spec in H.
-              congruence.
-        -- apply first_gamma_head_or_tail in Hfg.
-           inv Hfg.
-           ++ destruct Hfm as [Hsou Hcom].
-              eapply Hcom in H.
-              destruct H as [fiSet [Hnf Hli]]; auto.
-              congruence.
-           ++ destruct H.
-              destruct Hnu as [Hsou Hcom].
-              apply Hcom in H.
-              rewrite <- NtSet.mem_spec in H.
-              congruence.
-Qed.
+          -- inv Hin.
+  Qed.
 
-Lemma nullableGamma_correct :
-  forall g nu gamma,
-    nullable_set_for nu g
-    -> nullableGamma gamma nu = true
-       <-> nullable_gamma g gamma.
-Proof.
-  intros g nu gamma Hns.
-  split; [intros Hf | intros Hr].
-  - induction gamma as [| sym syms]; simpl in *; auto.
-    + destruct sym as [y | x].
-      * inv Hf.
-      * destruct (NtSet.mem x nu) eqn:Hmem.
-        -- constructor; auto.
-           destruct Hns as [Hsou Hcom].
-           apply Hsou.
-           rewrite <- NtSet.mem_spec; auto.
-        -- inv Hf.
-  - induction gamma as [| sym syms]; simpl in *; auto.
-    destruct sym as [y | x].
-    + exfalso.
-      eapply gamma_with_terminal_not_nullable with (gpre := nil); eauto.
-    + inv Hr.
-      destruct Hns as [Hsou Hcom].
-      apply Hcom in H1.
-      rewrite <- NtSet.mem_spec in H1.
-      rewrite H1; auto.
-Qed.
-      
-Lemma followLookahead_sound :
-  forall g la nu fo x gamma,
-    nullable_set_for nu g
-    -> follow_map_for fo g
-    -> In la (followLookahead x gamma nu fo)
-    -> nullable_gamma g gamma /\ follow_sym g la (NT x).
-Proof.
-  intros g la nu fo x gamma Hns Hfm Hin.
-  unfold followLookahead in Hin.
-  destruct (nullableGamma gamma nu) eqn:Hng.
-  - split.
-    + eapply nullableGamma_correct; eauto.
-    + destruct (NtMap.find x fo) as [foSet |] eqn:Hfind.
-      * destruct Hfm as [Hsou Hcom].
-        eapply Hsou; eauto.
-        apply in_elements_iff_in_laSet; auto.
-      * inv Hin.
-  - inv Hin.
-Qed.
+  (* There's probably a way to shorten this *)
+  Lemma firstGamma_complete :
+    forall g la nu fi gamma,
+      nullable_set_for nu g
+      -> first_map_for fi g
+      -> first_gamma g la gamma
+      -> In la (firstGamma' gamma nu fi).
+  Proof.
+    intros g la nu fi gamma Hnu Hfm Hfg.
+    induction gamma as [| sym syms].
+    - simpl in *.
+      inv Hfg. (* LEMMA *)
+      symmetry in H.
+      apply app_cons_not_nil in H; inv H.
+    - destruct sym as [y | x]; simpl in *.
+      + apply first_gamma_terminal_head in Hfg; auto.
+      + destruct (NtSet.mem x nu) eqn:Hmem.
+        * (* x is in the nullable set, so we know it's nullable *)
+          destruct (NtMap.find x fi) as [fiSet |] eqn:Hfind.
+          -- apply in_or_app.
+             apply first_gamma_head_or_tail in Hfg.
+             inv Hfg.
+             ++ destruct Hfm as [Hsou Hcom].
+                eapply Hcom in H.
+                destruct H as [fiSet' [Hnf Hlin]]; auto.
+                left.
+                assert (fiSet = fiSet') by congruence; subst.
+                apply in_elements_iff_in_laSet; auto.
+             ++ destruct H.
+                right; auto.
+          -- simpl.
+             apply IHsyms.
+             apply first_gamma_head_or_tail in Hfg.
+             inv Hfg.
+             ++ destruct Hfm as [Hsou Hcom].
+                eapply Hcom in H.
+                destruct H as [fiSet' [Hnf Hli]]; auto.
+                congruence.
+             ++ destruct H; auto.
+        * destruct (NtMap.find x fi) as [fiSet |] eqn:Hfind.
+          -- apply first_gamma_head_or_tail in Hfg.
+             inv Hfg.
+             ++ destruct Hfm as [Hsou Hcom].
+                eapply Hcom in H.
+                destruct H as [fiSet' [Hnf Hli]]; auto.
+                assert (fiSet = fiSet') by congruence; subst.
+                apply in_elements_iff_in_laSet; auto.
+             ++ destruct H.
+                destruct Hnu as [Hsou Hcom].
+                apply Hcom in H.
+                rewrite <- NtSet.mem_spec in H.
+                congruence.
+          -- apply first_gamma_head_or_tail in Hfg.
+             inv Hfg.
+             ++ destruct Hfm as [Hsou Hcom].
+                eapply Hcom in H.
+                destruct H as [fiSet [Hnf Hli]]; auto.
+                congruence.
+             ++ destruct H.
+                destruct Hnu as [Hsou Hcom].
+                apply Hcom in H.
+                rewrite <- NtSet.mem_spec in H.
+                congruence.
+  Qed.
 
-Lemma fromLookaheadList_preserves_in :
-  forall xp la las,
-    In (xp, la) (fromLookaheadList xp las) <-> In la las.
-Proof.
-  intros xp la las.
-  split; intros Hin.
-  - induction las; simpl in *; auto.
-    inv Hin; auto.
-    inv H; auto.
-  - induction las; simpl in *; auto.
-    inv Hin; auto.
-Qed.
-
-Lemma fromLookaheadList_preserves_soundness :
-  forall g xp la las,
-    In (xp, la) (fromLookaheadList xp las)
-    -> (forall la', In la' las -> lookahead_for la' (lhs xp) (rhs xp) g)
-    -> lookahead_for la (lhs xp) (rhs xp) g.
-Proof.
-  intros g xp la las Hin Hcor.
-  apply Hcor.
-  eapply fromLookaheadList_preserves_in; eauto.
-Qed.
-
-Lemma firstEntries_sound :
-  forall g nu fi xp la,
-    nullable_set_for nu g
-    -> first_map_for fi g
-    -> In (xp, la) (firstEntries xp nu fi)
-    -> lookahead_for la (lhs xp) (rhs xp) g.
-Proof.
-  intros g nu fi xp la Hns Hfm Hin.
-  eapply fromLookaheadList_preserves_soundness; eauto.
-  intros la' Hin'.
-  left; eapply firstGamma_sound; eauto.
-Qed.
-
-Lemma followEntries_sound :
-  forall g nu fo xp la,
-    nullable_set_for nu g
-    -> follow_map_for fo g
-    -> In (xp, la) (followEntries xp nu fo)
-    -> lookahead_for la (lhs xp) (rhs xp) g.
-Proof.
-  intros g nu fo xp la Hns Hfm Hin.
-  eapply fromLookaheadList_preserves_soundness; eauto.
-  intros la' Hin'.
-  right; eapply followLookahead_sound; eauto.
-Qed.
+  Lemma nullableGamma_correct :
+    forall g nu gamma,
+      nullable_set_for nu g
+      -> nullableGamma gamma nu = true
+         <-> nullable_gamma g gamma.
+  Proof.
+    intros g nu gamma Hns.
+    split; [intros Hf | intros Hr].
+    - induction gamma as [| sym syms]; simpl in *; auto.
+      + destruct sym as [y | x].
+        * inv Hf.
+        * destruct (NtSet.mem x nu) eqn:Hmem.
+          -- constructor; auto.
+             destruct Hns as [Hsou Hcom].
+             apply Hsou.
+             rewrite <- NtSet.mem_spec; auto.
+          -- inv Hf.
+    - induction gamma as [| sym syms]; simpl in *; auto.
+      destruct sym as [y | x].
+      + exfalso.
+        eapply gamma_with_terminal_not_nullable with (gpre := nil); eauto.
+      + inv Hr.
+        destruct Hns as [Hsou Hcom].
+        apply Hcom in H1.
+        rewrite <- NtSet.mem_spec in H1.
+        rewrite H1; auto.
+  Qed.
   
-Lemma entriesForProd_sound :
-  forall g nu fi fo xp xp' la,
-    nullable_set_for nu g
-    -> first_map_for fi g
-    -> follow_map_for fo g
-    -> In (xp, la) (entriesForProd nu fi fo xp')
-    -> lookahead_for la (lhs xp) (rhs xp) g.
-Proof.
-  intros g nu fi fo xp xp' la Hns Hfi Hfo Hin.
-  pose proof Hin as Hin'.
-  apply entriesForProd_preserves_prod in Hin'; subst.
-  unfold entriesForProd in Hin.
-  apply in_app_or in Hin; destruct Hin.
-  - eapply firstEntries_sound; eauto.
-  - eapply followEntries_sound; eauto.
-Qed.
+  Lemma followLookahead_sound :
+    forall g la nu fo x gamma,
+      nullable_set_for nu g
+      -> follow_map_for fo g
+      -> In la (followLookahead x gamma nu fo)
+      -> nullable_gamma g gamma /\ follow_sym g la (NT x).
+  Proof.
+    intros g la nu fo x gamma Hns Hfm Hin.
+    unfold followLookahead in Hin.
+    destruct (nullableGamma gamma nu) eqn:Hng.
+    - split.
+      + eapply nullableGamma_correct; eauto.
+      + destruct (NtMap.find x fo) as [foSet |] eqn:Hfind.
+        * destruct Hfm as [Hsou Hcom].
+          eapply Hsou; eauto.
+          apply in_elements_iff_in_laSet; auto.
+        * inv Hin.
+    - inv Hin.
+  Qed.
 
-Lemma fromLookaheadList_preserves_list_completeness :
-  forall P xp la las,
-    P la
-    -> (forall la', P la' -> In la' las)
-    -> In (xp, la) (fromLookaheadList xp las).
-Proof.
-  intros P xp la las Hp Hcor.
-  apply fromLookaheadList_preserves_in; auto.
-Qed.
+  Lemma fromLookaheadList_preserves_in :
+    forall xp la las,
+      In (xp, la) (fromLookaheadList xp las) <-> In la las.
+  Proof.
+    intros xp la las.
+    split; intros Hin.
+    - induction las; simpl in *; auto.
+      inv Hin; auto.
+      inv H; auto.
+    - induction las; simpl in *; auto.
+      inv Hin; auto.
+  Qed.
 
-Lemma firstEntries_complete :
-  forall g nu fi xp la,
-    nullable_set_for nu g
-    -> first_map_for fi g
-    -> first_gamma g la (rhs xp)
-    -> In (xp, la) (firstEntries xp nu fi).
-Proof.
-  intros g nu fi xp la Hnu Hfi Hfg.
-  unfold firstEntries.
-  eapply fromLookaheadList_preserves_list_completeness with
-      (P := fun la => first_gamma g la (rhs xp)); auto.
-  intros la' Hfg'.
-  eapply firstGamma_complete; eauto.
-Qed.
+  Lemma fromLookaheadList_preserves_soundness :
+    forall g xp la las,
+      In (xp, la) (fromLookaheadList xp las)
+      -> (forall la', In la' las -> lookahead_for la' (lhs xp) (rhs xp) g)
+      -> lookahead_for la (lhs xp) (rhs xp) g.
+  Proof.
+    intros g xp la las Hin Hcor.
+    apply Hcor.
+    eapply fromLookaheadList_preserves_in; eauto.
+  Qed.
 
-Lemma followLookahead_complete :
-  forall g nu fo xp la,
-    nullable_set_for nu g
-    -> follow_map_for fo g
-    -> nullable_gamma g (rhs xp)
-    -> follow_sym g la (NT (lhs xp))
-    -> In la (followLookahead (lhs xp) (rhs xp) nu fo).
-Proof.
-  intros g nu fo xp la Hns Hfm Hng Hfs.
-  unfold followLookahead.
-  eapply nullableGamma_correct in Hng; eauto.
-  rewrite Hng.
-  destruct Hfm as [Hsou Hcom].
-  eapply Hcom in Hfs.
-  destruct Hfs as [xFollow [Hnf Hli]]; auto.
-  rewrite Hnf.
-  apply in_elements_iff_in_laSet; auto.
-Qed.
+  Lemma firstEntries_sound :
+    forall g nu fi xp la,
+      nullable_set_for nu g
+      -> first_map_for fi g
+      -> In (xp, la) (firstEntries xp nu fi)
+      -> lookahead_for la (lhs xp) (rhs xp) g.
+  Proof.
+    intros g nu fi xp la Hns Hfm Hin.
+    eapply fromLookaheadList_preserves_soundness; eauto.
+    intros la' Hin'.
+    left; eapply firstGamma_sound; eauto.
+  Qed.
 
-Lemma followEntries_complete :
-  forall g nu fo xp la,
-    nullable_set_for nu g
-    -> follow_map_for fo g
-    -> nullable_gamma g (rhs xp)
-    -> follow_sym g la (NT (lhs xp))
-    -> In (xp, la) (followEntries xp nu fo).
-Proof.
-  intros g nu fo xp la Hns Hfm Hng Hfs.
-  unfold followEntries.
-  apply fromLookaheadList_preserves_list_completeness with
-      (P := fun la => follow_sym g la (NT (lhs xp))); auto.
+  Lemma followEntries_sound :
+    forall g nu fo xp la,
+      nullable_set_for nu g
+      -> follow_map_for fo g
+      -> In (xp, la) (followEntries xp nu fo)
+      -> lookahead_for la (lhs xp) (rhs xp) g.
+  Proof.
+    intros g nu fo xp la Hns Hfm Hin.
+    eapply fromLookaheadList_preserves_soundness; eauto.
+    intros la' Hin'.
+    right; eapply followLookahead_sound; eauto.
+  Qed.
+  
+  Lemma entriesForProd_sound :
+    forall g nu fi fo xp xp' la,
+      nullable_set_for nu g
+      -> first_map_for fi g
+      -> follow_map_for fo g
+      -> In (xp, la) (entriesForProd nu fi fo xp')
+      -> lookahead_for la (lhs xp) (rhs xp) g.
+  Proof.
+    intros g nu fi fo xp xp' la Hns Hfi Hfo Hin.
+    pose proof Hin as Hin'.
+    apply entriesForProd_preserves_prod in Hin'; subst.
+    unfold entriesForProd in Hin.
+    apply in_app_or in Hin; destruct Hin.
+    - eapply firstEntries_sound; eauto.
+    - eapply followEntries_sound; eauto.
+  Qed.
+
+  Lemma fromLookaheadList_preserves_list_completeness :
+    forall P xp la las,
+      P la
+      -> (forall la', P la' -> In la' las)
+      -> In (xp, la) (fromLookaheadList xp las).
+  Proof.
+    intros P xp la las Hp Hcor.
+    apply fromLookaheadList_preserves_in; auto.
+  Qed.
+
+  Lemma firstEntries_complete :
+    forall g nu fi xp la,
+      nullable_set_for nu g
+      -> first_map_for fi g
+      -> first_gamma g la (rhs xp)
+      -> In (xp, la) (firstEntries xp nu fi).
+  Proof.
+    intros g nu fi xp la Hnu Hfi Hfg.
+    unfold firstEntries.
+    eapply fromLookaheadList_preserves_list_completeness with
+        (P := fun la => first_gamma g la (rhs xp)); auto.
+    intros la' Hfg'.
+    eapply firstGamma_complete; eauto.
+  Qed.
+
+  Lemma followLookahead_complete :
+    forall g nu fo xp la,
+      nullable_set_for nu g
+      -> follow_map_for fo g
+      -> nullable_gamma g (rhs xp)
+      -> follow_sym g la (NT (lhs xp))
+      -> In la (followLookahead (lhs xp) (rhs xp) nu fo).
+  Proof.
+    intros g nu fo xp la Hns Hfm Hng Hfs.
+    unfold followLookahead.
+    eapply nullableGamma_correct in Hng; eauto.
+    rewrite Hng.
+    destruct Hfm as [Hsou Hcom].
+    eapply Hcom in Hfs.
+    destruct Hfs as [xFollow [Hnf Hli]]; auto.
+    rewrite Hnf.
+    apply in_elements_iff_in_laSet; auto.
+  Qed.
+
+  Lemma followEntries_complete :
+    forall g nu fo xp la,
+      nullable_set_for nu g
+      -> follow_map_for fo g
+      -> nullable_gamma g (rhs xp)
+      -> follow_sym g la (NT (lhs xp))
+      -> In (xp, la) (followEntries xp nu fo).
+  Proof.
+    intros g nu fo xp la Hns Hfm Hng Hfs.
+    unfold followEntries.
+    apply fromLookaheadList_preserves_list_completeness with
+        (P := fun la => follow_sym g la (NT (lhs xp))); auto.
     intros la' Hfs'.
     eapply followLookahead_complete; eauto.
-Qed.
+  Qed.
 
-Lemma entriesForProd_complete :
-  forall g nu fi fo xp la,
-    nullable_set_for nu g
-    -> first_map_for fi g
-    -> follow_map_for fo g
-    -> lookahead_for la (lhs xp) (rhs xp) g
-    -> In (xp, la) (entriesForProd nu fi fo xp).
-Proof.
-  intros g nu fi fo xp la Hnu Hfi Hfo Hlf.
-  unfold entriesForProd.
-  apply in_or_app; inv Hlf.
-  - left; eapply firstEntries_complete; eauto.
-  - destruct H.
-    right; eapply followEntries_complete; eauto.
-Qed.
+  Lemma entriesForProd_complete :
+    forall g nu fi fo xp la,
+      nullable_set_for nu g
+      -> first_map_for fi g
+      -> follow_map_for fo g
+      -> lookahead_for la (lhs xp) (rhs xp) g
+      -> In (xp, la) (entriesForProd nu fi fo xp).
+  Proof.
+    intros g nu fi fo xp la Hnu Hfi Hfo Hlf.
+    unfold entriesForProd.
+    apply in_or_app; inv Hlf.
+    - left; eapply firstEntries_complete; eauto.
+    - destruct H.
+      right; eapply followEntries_complete; eauto.
+  Qed.
 
-Lemma mkEntries'_correct :
-  forall g nu fi fo,
-    nullable_set_for nu g
-    -> first_map_for fi g
-    -> follow_map_for fo g
-    -> forall xps es,
-        mkEntries' nu fi fo xps = es
-        -> entries_correct_wrt_productions es xps g.
-Proof.
-  intros g nu fi fo Hnu Hfi Hfo xps.
-  induction xps as [| xp xps]; intros es Hmk; simpl in *; subst.
-  - apply empty_entries_correct_wrt_empty_productions.
-  - unfold entries_correct_wrt_productions.
-    intros xp' la.
-    split; [intros Hin | intros [Hin Hlf]].
-    + apply in_app_or in Hin.
-      destruct Hin.
-      * split.
-        -- left; apply entriesForProd_preserves_prod in H; auto.
-        -- eapply entriesForProd_sound; eauto.
-      * specialize IHxps with
-          (es := mkEntries' nu fi fo xps).
-        unfold entries_correct_wrt_productions in IHxps.
-        apply IHxps in H; auto.
-        destruct H as [Hin Hlf].
-        split; auto.
-        right; auto.
-    + subst.
-      apply in_or_app.
-      inv Hin.
-      * left.
-        eapply entriesForProd_complete; eauto.
-      * right.
-        specialize (IHxps (mkEntries' nu fi fo xps)).
-        unfold entries_correct_wrt_productions in IHxps.
-        apply IHxps; auto.
-Qed.
+  Lemma mkEntries'_correct :
+    forall g nu fi fo,
+      nullable_set_for nu g
+      -> first_map_for fi g
+      -> follow_map_for fo g
+      -> forall xps es,
+          mkEntries' nu fi fo xps = es
+          -> entries_correct_wrt_productions es xps g.
+  Proof.
+    intros g nu fi fo Hnu Hfi Hfo xps.
+    induction xps as [| xp xps]; intros es Hmk; simpl in *; subst.
+    - apply empty_entries_correct_wrt_empty_productions.
+    - unfold entries_correct_wrt_productions.
+      intros xp' la.
+      split; [intros Hin | intros [Hin Hlf]].
+      + apply in_app_or in Hin.
+        destruct Hin.
+        * split.
+          -- left; apply entriesForProd_preserves_prod in H; auto.
+          -- eapply entriesForProd_sound; eauto.
+        * specialize IHxps with
+              (es := mkEntries' nu fi fo xps).
+          unfold entries_correct_wrt_productions in IHxps.
+          apply IHxps in H; auto.
+          destruct H as [Hin Hlf].
+          split; auto.
+          right; auto.
+      + subst.
+        apply in_or_app.
+        inv Hin.
+        * left.
+          eapply entriesForProd_complete; eauto.
+        * right.
+          specialize (IHxps (mkEntries' nu fi fo xps)).
+          unfold entries_correct_wrt_productions in IHxps.
+          apply IHxps; auto.
+  Qed.
   
-Theorem mkEntries_correct :
-  forall (g  : grammar)
-         (nu : NtSet.t)
-         (fi : first_map)
-         (fo : follow_map) 
-         (es : list table_entry),
-    nullable_set_for nu g
-    -> first_map_for fi g
-    -> follow_map_for fo g
-    -> mkEntries nu fi fo g = es
-    -> entries_correct es g.
-Proof.
-  intros g nu fi fo es Hnu Hfi Hfo Hmk.
-  apply invariant_iff_entries_correct.
-  unfold mkEntries in Hmk.
-  eapply mkEntries'_correct; eauto.
-Qed.
+  Theorem mkEntries_correct :
+    forall (g  : grammar)
+           (nu : NtSet.t)
+           (fi : first_map)
+           (fo : follow_map) 
+           (es : list table_entry),
+      nullable_set_for nu g
+      -> first_map_for fi g
+      -> follow_map_for fo g
+      -> mkEntries nu fi fo g = es
+      -> entries_correct es g.
+  Proof.
+    intros g nu fi fo es Hnu Hfi Hfo Hmk.
+    apply invariant_iff_entries_correct.
+    unfold mkEntries in Hmk.
+    eapply mkEntries'_correct; eauto.
+  Qed.
 
 End EntryProofsFn.
 
